src/program_proof/pav/server.v
@@ -1,4 +1,5 @@
 From Perennial.program_proof Require Import grove_prelude.
+From Goose.github_com.mit_pdos.pav Require Import kt.
 
 Section inv.
 Context `{!heapGS Σ}.
@@ -6,3 +7,24 @@ Definition serv_sigpred (γ : gname) : (list w8 → iProp Σ) :=
   (* TODO: fill in. *)
   λ data, True%I.
 End inv.
+
+Module Server.
+Definition t : Type. Admitted.
+
+Section defs.
+Context `{!heapGS Σ}.
+Definition own (ptr : loc) (obj : t) : iProp Σ. Admitted.
+End defs.
+End Server.
+
+Section specs.
+Context `{!heapGS Σ}.
+Lemma wp_newServer :
+  {{{ True }}}
+  newServer #()
+  {{{
+    ptr_serv (serv : Server.t) (sigPk vrfPk : loc), RET (#ptr_serv, #sigPk, #vrfPk);
+    "Hown_serv" ∷ Server.own ptr_serv serv
+  }}}.
+Proof. Admitted.
+End specs.
