src/program_proof/pav/advrpc.v
@@ -1,0 +1,50 @@
+From Perennial.program_proof Require Import grove_prelude.
+From Goose.github_com.mit_pdos.pav Require Import advrpc.
+
+Module Server.
+Definition t : Type. Admitted.
+
+Section defs.
+Context `{!heapGS Σ}.
+Definition own (ptr : loc) (obj : t) : iProp Σ. Admitted.
+End defs.
+End Server.
+
+Module Client.
+Definition t : Type. Admitted.
+
+Section defs.
+Context `{!heapGS Σ}.
+Definition own (ptr : loc) (obj : t) : iProp Σ. Admitted.
+End defs.
+End Client.
+
+Section specs.
+Context `{!heapGS Σ}.
+Lemma wp_NewServer (handlers : loc) :
+  {{{ True }}}
+  NewServer #handlers
+  {{{
+    ptr_serv serv, RET #ptr_serv;
+    "Hown_serv" ∷ Server.own ptr_serv serv
+  }}}.
+Proof. Admitted.
+
+Lemma wp_Server__Serve ptr_serv serv (addr : w64) :
+  {{{
+    "Hown_serv" ∷ Server.own ptr_serv serv
+  }}}
+  Server__Serve #ptr_serv #addr
+  {{{ RET #(); True }}}.
+Proof. Admitted.
+
+Lemma wp_Dial (addr : w64) :
+  {{{ True }}}
+  Dial #addr
+  {{{
+    ptr_cli cli, RET #ptr_cli;
+    "Hown_cli" ∷ Client.own ptr_cli cli
+  }}}.
+Proof. Admitted.
+
+End specs.
