src/program_proof/pav/basictest.v
@@ -1,1 +1,108 @@
+From Perennial.program_proof Require Import grove_prelude.
 From Goose.github_com.mit_pdos.pav Require Import kt.
+
+From Perennial.program_proof.pav Require Import advrpc auditor core client rpc server.
+From Perennial.program_proof Require Import std_proof.
+
+Section proof.
+Context `{!heapGS Σ, !pavG Σ}.
+
+Lemma wp_testBasic (servAddr adtr0Addr adtr1Addr : w64) :
+  {{{ True }}}
+  testBasic #servAddr #adtr0Addr #adtr1Addr
+  {{{ RET #(); True }}}.
+Proof.
+  rewrite /testBasic.
+  iIntros (Φ) "_ HΦ".
+
+  (* set up server and auditors. *)
+  wp_apply wp_newServer. iIntros (????). iNamed 1.
+  wp_pures.
+  wp_apply (wp_newRpcServer with "Hown_serv"). iIntros (??). iNamed 1.
+  wp_apply (wp_Server__Serve with "Hown_rpcserv").
+  wp_apply wp_newAuditor. iIntros (?????). iNamedSuffix 1 "0".
+  wp_apply (wp_newRpcAuditor with "[$Hown_adtr0]"). iIntros (??). iNamed 1.
+  wp_apply (wp_Server__Serve with "Hown_rpcserv").
+  wp_apply wp_newAuditor. iIntros (?????). iNamedSuffix 1 "1".
+  wp_apply (wp_newRpcAuditor with "[$Hown_adtr1]"). iIntros (??). iNamed 1.
+  wp_apply (wp_Server__Serve with "Hown_rpcserv").
+  wp_apply wp_Sleep.
+
+  (* alice put. *)
+  wp_apply wp_newClient. iIntros (??????). iNamedSuffix 1 "_al".
+  wp_apply wp_SliceSingleton; [val_ty|]. iIntros (?) "Hpk0".
+  iDestruct (slice.own_slice_to_small with "Hpk0") as "Hpk0".
+  wp_apply (wp_Client__Put with "[$Hown_cli_al Hpk0]").
+  { instantiate (1:=[_]). iFrame "Hpk0". }
+  iIntros (ep0 ? err0) "H /=". iNamedSuffix "H" "_al".
+  wp_loadField. iClear "Herr_al". destruct err0.(clientErr.err).
+  { wp_apply wp_Assume_false. }
+  wp_apply wp_Assume. iIntros "_ /=". iNamedSuffix "H" "_al".
+
+  (* update auditors. *)
+  wp_apply wp_Dial. iIntros (??). iNamedSuffix 1 "0".
+  wp_apply wp_Dial. iIntros (??). iNamedSuffix 1 "1".
+  wp_apply wp_Dial. iIntros (??). iNamedSuffix 1 "2".
+  wp_apply (wp_callServAudit with "Hown_cli0").
+  iIntros (?? err1) "H". iNamedSuffix "H" "0". destruct err1.
+  { wp_apply wp_Assume_false. }
+  simpl. iNamedSuffix "H" "0". wp_apply wp_Assume. iIntros "_".
+  wp_apply (wp_callServAudit with "Hown_cli0").
+  iIntros (?? err2) "H". iNamedSuffix "H" "0". destruct err2.
+  { wp_apply wp_Assume_false. }
+  simpl. iNamedSuffix "H" "1". wp_apply wp_Assume. iIntros "_".
+  wp_apply (wp_callAdtrUpdate with "[$Hown_cli1 $Hown_upd0]").
+  iIntros (?) "H". iEval (rewrite /named) in "H".
+  iDestruct "H" as "[Hown_cli1 Hown_upd0]".
+  wp_apply wp_Assume. iIntros "_".
+  wp_apply (wp_callAdtrUpdate with "[$Hown_cli1 $Hown_upd1]").
+  iIntros (?) "H". iEval (rewrite /named) in "H".
+  iDestruct "H" as "[Hown_cli1 Hown_upd1]".
+  wp_apply wp_Assume. iIntros "_".
+  wp_apply (wp_callAdtrUpdate with "[$Hown_cli2 $Hown_upd0]").
+  iIntros (?) "H". iEval (rewrite /named) in "H".
+  iDestruct "H" as "[Hown_cli2 Hown_upd0]".
+  wp_apply wp_Assume. iIntros "_".
+  wp_apply (wp_callAdtrUpdate with "[$Hown_cli2 $Hown_upd1]").
+  iIntros (?) "H". iEval (rewrite /named) in "H".
+  iDestruct "H" as "[Hown_cli2 Hown_upd1]".
+  wp_apply wp_Assume. iIntros "_".
+
+  (* bob get. *)
+  wp_apply wp_newClient. iIntros (??????). iNamedSuffix 1 "_bob".
+  wp_apply (wp_Client__Get with "Hown_cli_bob").
+  iIntros (is_reg ?? ep1 ? err7) "H /=". iNamedSuffix "H" "_bob".
+  wp_loadField. iClear "Herr_bob". destruct err7.(clientErr.err).
+  { wp_apply wp_Assume_false. }
+  wp_apply wp_Assume. iIntros "_". wp_apply wp_Assume. iIntros "%Heq_ep /=".
+  iNamedSuffix "H" "_bob". iRename "H" into "Hreg".
+
+  (* alice and bob audit. *)
+  wp_apply (wp_Client__Audit with "[$Hown_cli_al $Hsl_adtrPk0 $His_adtrPk0]").
+  iIntros (? err8) "H /=". iNamedSuffix "H" "_al".
+  wp_loadField. iClear "Herr_al". destruct err8.(clientErr.err).
+  { wp_apply wp_Assume_false. }
+  wp_apply wp_Assume. iIntros "_ /=". iNamedSuffix "H" "_al0".
+  wp_apply (wp_Client__Audit with "[$Hown_cli_al $Hsl_adtrPk1 $His_adtrPk1]").
+  iIntros (? err9) "H /=". iNamedSuffix "H" "_al".
+  wp_loadField. iClear "Herr_al". destruct err9.(clientErr.err).
+  { wp_apply wp_Assume_false. }
+  wp_apply wp_Assume. iIntros "_ /=". iNamedSuffix "H" "_al1".
+  wp_apply (wp_Client__Audit with "[$Hown_cli_bob $Hsl_adtrPk0 $His_adtrPk0]").
+  iIntros (? err10) "H /=". iNamedSuffix "H" "_bob".
+  wp_loadField. iClear "Herr_bob". destruct err10.(clientErr.err).
+  { wp_apply wp_Assume_false. }
+  wp_apply wp_Assume. iIntros "_ /=". iNamedSuffix "H" "_bob0".
+  wp_apply (wp_Client__Audit with "[$Hown_cli_bob $Hsl_adtrPk1 $His_adtrPk1]").
+  iIntros (? err11) "H /=". iNamedSuffix "H" "_bob".
+  wp_loadField. iClear "Herr_bob". destruct err11.(clientErr.err).
+  { wp_apply wp_Assume_false. }
+  wp_apply wp_Assume. iIntros "_ /=". iNamedSuffix "H" "_bob1".
+
+  (* main part: proving the pk's are equal. *)
+  iClear "Hsl_adtrPk0 His_adtrPk0 Hsl_adtrPk1 His_adtrPk1 Hown_cli0
+    Hown_cli1 Hown_cli2 Hown_upd0 Hown_upd1 Hown_cli_al Hown_cli_bob".
+  case_bool_decide; [|done]. simplify_eq/=.
+Admitted.
+
+End proof.
