src/program_proof/pav/rpc.v
@@ -1,0 +1,57 @@
+From Perennial.program_proof Require Import grove_prelude.
+From Goose.github_com.mit_pdos.pav Require Import kt.
+
+From Perennial.program_proof.pav Require Import auditor advrpc client core serde server.
+
+Section specs.
+Context `{!heapGS Σ, !pavG Σ}.
+Lemma wp_newRpcServer ptr_serv serv :
+  {{{
+    "Hown_serv" ∷ server.Server.own ptr_serv serv
+  }}}
+  newRpcServer #ptr_serv
+  {{{
+    ptr_rpcserv rpcserv, RET #ptr_rpcserv;
+    "Hown_rpcserv" ∷ advrpc.Server.own ptr_rpcserv rpcserv
+  }}}.
+Proof. Admitted.
+
+Lemma wp_newRpcAuditor ptr_adtr adtr :
+  {{{
+    "Hown_adtr" ∷ Auditor.own ptr_adtr adtr
+  }}}
+  newRpcAuditor #ptr_adtr
+  {{{
+    ptr_rpcserv rpcserv, RET #ptr_rpcserv;
+    "Hown_rpcserv" ∷ advrpc.Server.own ptr_rpcserv rpcserv
+  }}}.
+Proof. Admitted.
+
+Lemma wp_callServAudit ptr_cli cli (ep : w64) :
+  {{{
+    "Hown_cli" ∷ advrpc.Client.own ptr_cli cli
+  }}}
+  callServAudit #ptr_cli #ep
+  {{{
+    ptr_upd upd (err : bool), RET (#ptr_upd, #err);
+    "Hown_cli" ∷ advrpc.Client.own ptr_cli cli ∗
+    if negb err then
+      "Hown_upd" ∷ UpdateProof.own ptr_upd upd
+    else True
+  }}}.
+Proof. Admitted.
+
+Lemma wp_callAdtrUpdate ptr_cli cli ptr_upd upd :
+  {{{
+    "Hown_cli" ∷ advrpc.Client.own ptr_cli cli ∗
+    "Hown_upd" ∷ UpdateProof.own ptr_upd upd
+  }}}
+  callAdtrUpdate #ptr_cli #ptr_upd
+  {{{
+    (err : bool), RET #err;
+    "Hown_cli" ∷ advrpc.Client.own ptr_cli cli ∗
+    "Hown_upd" ∷ UpdateProof.own ptr_upd upd
+  }}}.
+Proof. Admitted.
+
+End specs.
